examples old and new

LeanLion/QuickSort.lean
@@ -13,3 +13,167 @@ Our implementation of quicksort for lists follows the following steps:
 * Let `smaller` be the list of elements smaller (`≤`) than `pivot` and `larger` be the list of elements larger (`>`) than `pivot`.
 * Recursively sort `smaller` and `larger` lists and concatenate them with `pivot` in between.
 -/
+
+namespace Quicksort
+
+variable {α : Type}[LinearOrder α]
+
+def smaller (pivot : α) (l : List α) : List α :=
+  l.filter (fun x => x ≤  pivot)
+
+def larger (pivot : α) (l : List α) : List α :=
+  l.filter (fun x => x > pivot)
+
+def quickSort : List α → List α
+  | [] => []
+  | pivot :: l =>
+    have : (smaller pivot l).length < (pivot :: l).length := by
+      simp [List.length_cons]
+      apply Nat.succ_le_succ
+      apply List.length_filter_le
+    have : (larger pivot l).length < (pivot :: l).length := by
+      simp [List.length_cons]
+      apply Nat.succ_le_succ
+      apply List.length_filter_le
+    (quickSort (smaller pivot l)) ++ pivot :: (quickSort (larger pivot l))
+termination_by l => l.length
+
+theorem quickSort_nil : quickSort ([] : List α) = [] := by
+  rfl
+
+theorem quickSort_cons (pivot : α) (l : List α) :
+    quickSort (pivot :: l) = (quickSort (smaller pivot l)) ++
+    pivot :: (quickSort (larger pivot l)) := by
+  rfl
+
+theorem mem_iff_below_or_above_pivot (pivot : α) (l : List α)(x : α) :
+    x ∈ l ↔ x ∈ smaller pivot l ∨ x ∈ larger pivot l := by
+  apply Iff.intro
+  · intro h
+    by_cases h' : x ≤ pivot
+    · left
+      apply List.mem_filter_of_mem h
+      simp
+      assumption
+    · right
+      apply List.mem_filter_of_mem h
+      simp
+      apply lt_of_not_ge
+      assumption
+  · intro h
+    cases h
+    case mpr.inl h' =>
+      apply List.mem_of_mem_filter
+      assumption
+    case mpr.inr h' =>
+      exact List.mem_of_mem_filter h'
+
+theorem mem_iff_mem_quickSort (l: List α)(x : α) :
+    x ∈ l ↔ x ∈ quickSort l := by
+  match l with
+  | [] =>
+    simp [quickSort_nil]
+  | pivot :: l =>
+    simp [quickSort_cons]
+    rw [mem_iff_below_or_above_pivot pivot]
+    have : (smaller pivot l).length < (pivot :: l).length := by
+      simp [List.length_cons]
+      apply Nat.succ_le_succ
+      apply List.length_filter_le
+    have : (larger pivot l).length < (pivot :: l).length := by
+      simp [List.length_cons]
+      apply Nat.succ_le_succ
+      apply List.length_filter_le
+    let ihb := mem_iff_mem_quickSort (smaller pivot l)
+    let iha := mem_iff_mem_quickSort (larger pivot l)
+    rw [← ihb, ← iha]
+    aesop
+termination_by l.length
+
+inductive Sorted : List α → Prop
+  | nil : Sorted []
+  | singleton (x : α) : Sorted [x]
+  | step (x y : α) (l : List α) :
+    x ≤ y → Sorted (y :: l) → Sorted (x :: y :: l)
+
+theorem append_sorted (bound: α)(l₁ l₂ : List α) :
+  (∀ x ∈ l₁, x ≤ bound) → (∀ x ∈ l₂, bound ≤  x) → Sorted l₁ → Sorted l₂ → Sorted (l₁ ++ l₂) := by
+  intro h₁ h₂ s₁
+  induction s₁
+  case nil =>
+    simp
+  case singleton x =>
+    simp at h₁
+    intro s₂
+    cases s₂
+    case nil =>
+      apply Sorted.singleton
+    case singleton y =>
+      apply Sorted.step x y
+      · simp at h₂
+        trans bound <;> assumption
+      · apply Sorted.singleton
+    case step y z l hyz s =>
+      simp
+      apply Sorted.step x y
+      · trans bound
+        · assumption
+        · simp [List.mem_cons] at h₂
+          exact h₂.left
+      · exact Sorted.step y z l hyz s
+  case step x y l hxy _ ih =>
+    intro s₂
+    apply Sorted.step x y (l ++ l₂) hxy
+    rw [← List.cons_append]
+    apply ih
+    · simp [List.mem_cons]
+      simp [List.mem_cons] at h₁
+      apply And.intro
+      · apply h₁.right.left
+      · apply h₁.right.right
+    · exact s₂
+
+theorem quickSort_sorted (l : List α) : Sorted (quickSort l) := by
+  match l with
+    | [] =>
+      simp [quickSort_nil]
+      apply Sorted.nil
+    | pivot :: l =>
+      rw [quickSort_cons]
+      have : (smaller pivot l).length < (pivot :: l).length := by
+        simp [List.length_cons]
+        apply Nat.succ_le_succ
+        apply List.length_filter_le
+      have : (larger pivot l).length < (pivot :: l).length := by
+        simp [List.length_cons]
+        apply Nat.succ_le_succ
+        apply List.length_filter_le
+      let ihb := quickSort_sorted (smaller pivot l)
+      let iha := quickSort_sorted (larger pivot l)
+      apply append_sorted pivot
+      · intro x
+        rw [← mem_iff_mem_quickSort]
+        intro h
+        let lem := List.of_mem_filter h
+        simp at lem
+        assumption
+      · simp
+        intro x
+        rw [← mem_iff_mem_quickSort]
+        intro h
+        let lem := List.of_mem_filter h
+        simp at lem
+        apply le_of_lt
+        assumption
+      · assumption
+      · apply append_sorted pivot [pivot] (quickSort (larger pivot l))
+        · simp
+        · intro x h
+          rw [← mem_iff_mem_quickSort] at h
+          let lem := List.of_mem_filter h
+          simp at lem
+          apply le_of_lt
+          assumption
+        · apply Sorted.singleton
+        · assumption
+termination_by l.length
