LeanLion/MetaExamples.lean
@@ -1,0 +1,46 @@
+import Lean
+
+open Lean Meta Elab Term
+
+macro "[" y:term "forr" x:ident "in" l:term "]" : term => do
+  `(List.map (fun $x => $y) $l)
+
+#eval [x * x forr x in [1, 2, 3, 4, 5]]
+
+elab "[" y:term "forrr" x:ident "in" l:term "]" : term => do
+  let lExpr ← elabTerm l none
+  match ← inferType lExpr with
+  | .app (.const name _) _ =>
+    match name with
+    | `List =>
+      let stx ← `(List.map (fun $x => $y) $l)
+      elabTerm stx none
+    | ``Array =>
+      let stx ← `(Array.toList (Array.map (fun $x => $y) $l))
+      elabTerm stx none
+    | _ => throwError s!"expected a list or array, got {name}"
+  | _ => throwError s!"expected a list or array, got {← ppExpr lExpr}"
+
+
+#eval [x * x forrr x in [2, 3]]
+
+declare_syntax_cat python_for
+syntax "for#" ident "in" term : python_for
+
+syntax "[" term python_for* "]" : term
+
+macro_rules
+| `([ $y:term $l:python_for ]) => do
+  match l with
+  | `(python_for| for# $x:ident in $l) => do
+    `(List.map (fun $x => $y) $l)
+  | _ => Macro.throwUnsupported
+| `([ $y:term $ls:python_for* $l:python_for]) => do
+  let init ← `([ $y:term $ls:python_for* ])
+  match l with
+  | `(python_for| for# $x:ident in $l) => do
+    `(List.bind $l (fun $x => $init))
+  | _ => Macro.throwUnsupported
+
+#eval [x * x for# x in [1, 2, 3, 4, 5]]
+#eval [x * x for# x in l for# l in [[1, 5, 2], [3, 4, 5]]]
